omni/LibSepVar.v
@@ -1,0 +1,168 @@
+(****************************************************************
+* Representation of Variables as Strings                        *
+* Utility Functions                                             *
+****************************************************************)
+
+Set Implicit Arguments.
+From TLC Require Export LibString LibList LibCore.
+Open Scope string_scope.
+
+
+(* ########################################################### *)
+(* ########################################################### *)
+(* ########################################################### *)
+(** * Representation of Program Variables *)
+
+(** This file contains definitions, lemmas, tactics and notations for
+    manipulating program variables and list of program variables. *)
+
+
+(* ########################################################### *)
+(** ** Representation of Variables *)
+
+(** Variables are represented as strings *)
+
+Definition var : Type := string.
+
+(** The boolean function [var_eq s1 s2] compares two variables. *)
+
+Definition var_eq (s1:var) (s2:var) : bool :=
+  if String.string_dec s1 s2 then true else false.
+
+(** The boolean function [var_eq s1 s2] returns [true] iff the
+    equality [v1 = v2] holds. *)
+
+Lemma var_eq_spec : forall s1 s2,
+  var_eq s1 s2 = isTrue (s1 = s2).
+Proof using.
+  intros. unfold var_eq. case_if; rew_bool_eq~.
+Qed.
+
+Global Opaque var.
+
+
+(* ########################################################### *)
+(** ** Tactic [case_var] *)
+
+(** The tactic [case_var] performs case analysis on expressions of the
+    form [if var_eq x y then .. else ..] that appear in the goal. *)
+
+Tactic Notation "case_var" :=
+  repeat rewrite var_eq_spec in *; repeat case_if.
+
+Tactic Notation "case_var" "~" :=
+  case_var; auto_tilde.
+
+Tactic Notation "case_var" "*" :=
+  case_var; auto_star.
+
+
+(* ########################################################### *)
+(* ########################################################### *)
+(* ########################################################### *)
+(** * Representation of List of Variables *)
+
+(* ########################################################### *)
+(** ** Definition of Distinct Variables *)
+
+(** [vars] is the type of a list of variables *)
+
+Definition vars : Type := list var.
+
+(** [var_fresh y xs] asserts that [y] does not belong to the list [xs] *)
+
+Definition var_fresh (y:var) (xs:vars) : Prop :=
+  ~ mem y xs.
+
+(** The following lemma asserts that if [x] is a variable in the list [xs],
+    and [y] is fresh from this list [xs], then [y] is not equal to [x]. *)
+
+Lemma var_fresh_mem_inv : forall y x xs,
+  var_fresh x xs ->
+  mem y xs ->
+  x <> y.
+Proof using. introv H M N. unfolds var_fresh. subst*. Qed.
+
+
+(* ########################################################### *)
+(** ** Generation of [n] Distinct Variables *)
+
+(** [nat_to_var n] converts [nat] values into distinct [name] values. *)
+
+(* LATER: make the implementation more optimized by using more than one
+   character. *)
+
+Definition dummy_char :=
+  Ascii.ascii_of_nat 0%nat.
+
+Fixpoint nat_to_var (n:nat) : var :=
+  match n with
+  | O => String.EmptyString
+  | S n' => String.String dummy_char (nat_to_var n')
+  end.
+
+Lemma injective_nat_to_var :
+  injective nat_to_var.
+Proof using.
+  intros n. induction n as [|n']; intros m E; destruct m as [|m']; tryfalse.
+  { auto. }
+  { inverts E. fequals~. }
+Qed.
+
+(** [var_seq i n] generates a list of variables [x1;x2;..;xn] with [x1=i] and
+    [xn=i+n-1]. The ability to start at a given offset is sometimes useful. *)
+
+Fixpoint var_seq (start:nat) (nb:nat) : vars :=
+  match nb with
+  | O => nil
+  | S nb' => (nat_to_var start) :: var_seq (S start) nb'
+  end.
+
+(** The properties of [var_seq] are stated next. They assert that this
+    function produce the expected number of variables, that the variables
+    are pairwise distinct *)
+
+Section Var_seq.
+Implicit Types start nb : nat.
+
+Lemma var_fresh_var_seq_lt : forall (x:nat) start nb,
+  (x < start)%nat ->
+  var_fresh (nat_to_var x) (var_seq start nb).
+Proof using.
+  intros. unfold var_fresh. gen start. induction nb; simpl; introv N; rew_listx.
+  { auto. }
+  { simpl. case_var. rew_logic. split.
+    { intros E. lets: injective_nat_to_var E. math. }
+    { applys IHnb. math. } }
+Qed.
+
+Lemma var_fresh_var_seq_ge : forall (x:nat) start nb,
+  (x >= start+nb)%nat ->
+  var_fresh (nat_to_var x) (var_seq start nb).
+Proof using.
+  intros. unfold var_fresh. gen start. induction nb; simpl; introv N; rew_listx.
+  { auto. }
+  { simpl. case_var. rew_logic. split.
+    { intros E. lets: injective_nat_to_var E. math. }
+    { applys IHnb. math. } }
+Qed.
+
+Lemma noduplicates_var_seq : forall start nb,
+  LibList.noduplicates (var_seq start nb).
+Proof using.
+  intros. gen start. induction nb; intros; simpl; rew_listx.
+  { auto. }
+  { split.
+    { applys var_fresh_var_seq_lt. math. }
+    { auto. } }
+Qed.
+
+Lemma length_var_seq : forall start nb,
+  length (var_seq start nb) = nb.
+Proof using.
+  intros. gen start. induction nb; simpl; intros.
+  { auto. } { rew_list. rewrite~ IHnb. }
+Qed.
+
+End Var_seq.
+
