omni/SepLogicCommon.v
@@ -1,0 +1,357 @@
+(****************************************************************
+* Imperative Lambda-calculus                                    *
+* Separation Logic Heap Predicates                              *
+*****************************************************************)
+
+Set Implicit Arguments.
+Require Export Syntax.
+
+Implicit Types f : var.
+Implicit Types b : bool.
+Implicit Types p : loc.
+Implicit Types n : int.
+Implicit Types v w r vf vx : val.
+Implicit Types t : trm.
+Implicit Types s : state.
+Implicit Types h : heap.
+Implicit Types P : Prop.
+Implicit Types H : hprop.
+Implicit Types Q : val->hprop.
+
+
+(** [Syntax.v] already contains the definition of [heap], [hprop],
+    and of the entailment relations. *)
+
+
+(* ########################################################### *)
+(* ########################################################### *)
+(* ########################################################### *)
+(** * Construction of Separation Logic Predicates *)
+
+(* ########################################################### *)
+(** ** Core Heap Predicates *)
+
+(** Core heap predicates, and their associated notations:
+
+    - [\[]] denotes the empty heap predicate
+    - [\[P]] denotes a pure fact
+    - [p ~~> v] denotes a singleton heap
+    - [H1 \* H2] denotes the separating conjunction
+    - [H1 \-* H2] denotes the magic wand
+    - [Q1 \--* Q2] denotes the magic wand on postconditions
+    - [Q1 \*+ H2] denotes the separating conjunction extending a postcondition
+    - [\exists x, H] denotes an existential
+    - [\forall x, H] denotes a universal. *)
+
+Definition hempty : hprop :=
+  fun h => (h = Fmap.empty).
+
+Definition hsingle (p:loc) (v:val) : hprop :=
+  fun h => (h = Fmap.single p v).
+
+Definition hstar (H1 H2 : hprop) : hprop :=
+  fun h => exists h1 h2, H1 h1
+                              /\ H2 h2
+                              /\ Fmap.disjoint h1 h2
+                              /\ h = Fmap.union h1 h2.
+
+Definition hexists A (J:A->hprop) : hprop :=
+  fun h => exists x, J x h.
+
+Definition hforall (A : Type) (J : A -> hprop) : hprop :=
+  fun h => forall x, J x h.
+
+Definition hpure (P:Prop) : hprop := (* encoded as [\exists (p:P), \[]] *)
+  hexists (fun (p:P) => hempty).
+
+Declare Scope hprop_scope.
+Open Scope hprop_scope.
+
+Notation "\[]" := (hempty)
+  (at level 0) : hprop_scope.
+
+Notation "\[ P ]" := (hpure P)
+  (at level 0, format "\[ P ]") : hprop_scope.
+
+Notation "p '~~>' v" := (hsingle p v) (at level 32) : hprop_scope.
+
+Notation "H1 '\*' H2" := (hstar H1 H2)
+  (at level 41, right associativity) : hprop_scope.
+
+Notation "Q \*+ H" := (fun x => hstar (Q x) H)
+  (at level 40) : hprop_scope.
+
+Notation "'\exists' x1 .. xn , H" :=
+  (hexists (fun x1 => .. (hexists (fun xn => H)) ..))
+  (at level 39, x1 binder, H at level 50, right associativity,
+   format "'[' '\exists' '/ '  x1  ..  xn , '/ '  H ']'") : hprop_scope.
+
+Notation "'\forall' x1 .. xn , H" :=
+  (hforall (fun x1 => .. (hforall (fun xn => H)) ..))
+  (at level 39, x1 binder, H at level 50, right associativity,
+   format "'[' '\forall' '/ '  x1  ..  xn , '/ '  H ']'") : hprop_scope.
+
+Definition hwand (H1 H2:hprop) : hprop :=
+  \exists H0, H0 \* \[ H1 \* H0 ==> H2 ].
+
+Notation "H1 \-* H2" := (hwand H1 H2)
+  (at level 43, right associativity) : hprop_scope.
+
+Definition qwand (Q1 Q2:val->hprop) : hprop :=
+  \forall v, (Q1 v) \-* (Q2 v).
+
+Notation "Q1 \--* Q2" := (qwand Q1 Q2)
+  (at level 43) : hprop_scope.
+
+
+(* ########################################################### *)
+(** ** Automation for Heap Equality and Heap Disjointness *)
+
+(** For goals asserting equalities between heaps, i.e., of the form [h1 = h2],
+    we set up automation so that it performs some tidying: substitution,
+    removal of empty heaps, normalization with respect to associativity. *)
+
+#[global] Hint Rewrite union_assoc union_empty_l union_empty_r : fmap.
+#[global] Hint Extern 1 (_ = _ :> heap) => subst; autorewrite with fmap.
+
+(** For goals asserting disjointness between heaps, i.e., of the form
+    [Fmap.disjoint h1 h2], we set up automation to perform simplifications:
+    substitution, exploit distributivity of the disjointness predicate over
+    unions of heaps, and exploit disjointness with empty heaps. The tactic
+    [jauto_set] used here comes from the TLC library; essentially, it destructs
+    conjunctions and existentials. *)
+
+#[global] Hint Resolve Fmap.disjoint_empty_l Fmap.disjoint_empty_r.
+#[global] Hint Rewrite disjoint_union_eq_l disjoint_union_eq_r : disjoint.
+#[global] Hint Extern 1 (Fmap.disjoint _ _) =>
+  subst; autorewrite with rew_disjoint in *; jauto_set.
+
+
+(* ########################################################### *)
+(** ** Properties of [hstar] *)
+
+Lemma hstar_intro : forall H1 H2 h1 h2,
+  H1 h1 ->
+  H2 h2 ->
+  Fmap.disjoint h1 h2 ->
+  (H1 \* H2) (Fmap.union h1 h2).
+Proof. intros. exists* h1 h2. Qed.
+
+Lemma hstar_comm : forall H1 H2,
+   H1 \* H2 = H2 \* H1.
+Proof.
+  unfold hprop, hstar. intros H1 H2. applys himpl_antisym.
+  { intros h (h1&h2&M1&M2&D&U).
+    rewrite* Fmap.union_comm_of_disjoint in U. exists* h2 h1. }
+  { intros h (h1&h2&M1&M2&D&U).
+    rewrite* Fmap.union_comm_of_disjoint in U. exists* h2 h1. }
+Qed.
+
+Lemma hstar_assoc : forall H1 H2 H3,
+  (H1 \* H2) \* H3 = H1 \* (H2 \* H3).
+Proof.
+  intros H1 H2 H3. applys himpl_antisym; intros h.
+  { intros (h'&h3&(h1&h2&M3&M4&D'&U')&M2&D&U). subst h'.
+    exists h1 (h2 \+ h3). splits*. { applys* hstar_intro. } }
+  { intros (h1&h'&M1&(h2&h3&M3&M4&D'&U')&D&U). subst h'.
+    exists (h1 \+ h2) h3. splits*. { applys* hstar_intro. } }
+Qed.
+
+Lemma hstar_hempty_l : forall H,
+  \[] \* H = H.
+Proof.
+  intros. applys himpl_antisym; intros h.
+  { intros (h1&h2&M1&M2&D&U). hnf in M1. subst. rewrite* Fmap.union_empty_l. }
+  { intros M. exists (@Fmap.empty loc val) h. splits*. { hnfs*. } }
+Qed.
+
+Lemma hstar_hexists : forall A (J:A->hprop) H,
+  (hexists J) \* H = hexists (fun x => (J x) \* H).
+Proof.
+  intros. applys himpl_antisym; intros h.
+  { intros (h1&h2&(x&M1)&M2&D&U). exists* x h1 h2. }
+  { intros (x&(h1&h2&M1&M2&D&U)). exists h1 h2. splits*. { exists* x. } }
+Qed.
+
+Lemma hstar_hforall : forall H A (J:A->hprop),
+  (hforall J) \* H ==> hforall (J \*+ H).
+Proof.
+  intros. intros h M. destruct M as (h1&h2&M1&M2&D&U). intros x. exists* h1 h2.
+Qed.
+
+Lemma himpl_frame_l : forall H2 H1 H1',
+  H1 ==> H1' ->
+  (H1 \* H2) ==> (H1' \* H2).
+Proof. introv W (h1&h2&?). exists* h1 h2. Qed.
+
+(** Additional, symmetric results, useful for tactics *)
+
+Lemma hstar_hempty_r : forall H,
+  H \* \[] = H.
+Proof.
+  applys neutral_r_of_comm_neutral_l. applys* hstar_comm. applys* hstar_hempty_l.
+Qed.
+
+Lemma himpl_frame_r : forall H1 H2 H2',
+  H2 ==> H2' ->
+  (H1 \* H2) ==> (H1 \* H2').
+Proof.
+  introv M. do 2 rewrite (@hstar_comm H1). applys* himpl_frame_l.
+Qed.
+
+
+(* ########################################################### *)
+(** ** Properties of [hpure] *)
+
+Lemma hstar_hpure_l : forall P H h,
+  (\[P] \* H) h = (P /\ H h).
+Proof.
+  intros. apply prop_ext. unfold hpure.
+  rewrite hstar_hexists. rewrite* hstar_hempty_l.
+  iff (p&M) (p&M). { split*. } { exists* p. }
+Qed.
+
+Lemma himpl_hstar_hpure_r : forall P H H',
+  P ->
+  (H ==> H') ->
+  H ==> (\[P] \* H').
+Proof. introv HP W. intros h K. rewrite* hstar_hpure_l. Qed.
+
+Lemma himpl_hstar_hpure_l : forall P H H',
+  (P -> H ==> H') ->
+  (\[P] \* H) ==> H'.
+Proof. introv W Hh. rewrite hstar_hpure_l in Hh. applys* W. Qed.
+
+
+(* ########################################################### *)
+(** ** Properties of [hexists] *)
+
+Lemma himpl_hexists_l : forall A H (J:A->hprop),
+  (forall x, J x ==> H) ->
+  (hexists J) ==> H.
+Proof. introv W. intros h (x&Hh). applys* W. Qed.
+
+Lemma himpl_hexists_r : forall A (x:A) H J,
+  (H ==> J x) ->
+  H ==> (hexists J).
+Proof. introv W. intros h. exists x. apply* W. Qed.
+
+Lemma himpl_hexists : forall A (J1 J2:A->hprop),
+  J1 ===> J2 ->
+  hexists J1 ==> hexists J2.
+Proof.
+  introv W. applys himpl_hexists_l. intros x. applys himpl_hexists_r W.
+Qed.
+
+
+(* ########################################################### *)
+(** ** Properties of [hforall] *)
+
+Lemma himpl_hforall_r : forall A (J:A->hprop) H,
+  (forall x, H ==> J x) ->
+  H ==> (hforall J).
+Proof. introv M. intros h Hh x. apply* M. Qed.
+
+Lemma himpl_hforall_l : forall A x (J:A->hprop) H,
+  (J x ==> H) ->
+  (hforall J) ==> H.
+Proof. introv M. intros h Hh. apply* M. Qed.
+
+Lemma himpl_hforall : forall A (J1 J2:A->hprop),
+  J1 ===> J2 ->
+  hforall J1 ==> hforall J2.
+Proof.
+  introv W. applys himpl_hforall_r. intros x. applys himpl_hforall_l W.
+Qed.
+
+
+(* ########################################################### *)
+(** ** Basic Tactics for Simplifying Entailments *)
+
+(** [xsimpl] performs immediate simplifications on entailment relations.
+    For a more powerful version of [xsimpl], see the course
+    Separation Logic Foundations, or the implementation of the CFML tool. *)
+
+#[global] Hint Rewrite hstar_assoc hstar_hempty_l hstar_hempty_r : hstar.
+
+Tactic Notation "xsimpl" :=
+  try solve [ apply qimpl_refl ];
+  try match goal with |- _ ===> _ => intros ? end;
+  autorewrite with hstar; repeat match goal with
+  | |- ?H \* _ ==> ?H \* _ => apply himpl_frame_r
+  | |- _ \* ?H ==> _ \* ?H => apply himpl_frame_l
+  | |- _ \* ?H ==> ?H \* _ => rewrite hstar_comm; apply himpl_frame_r
+  | |- ?H \* _ ==> _ \* ?H => rewrite hstar_comm; apply himpl_frame_l
+  | |- ?H ==> ?H => apply himpl_refl
+  | |- ?H ==> ?H' => is_evar H'; apply himpl_refl end.
+
+Tactic Notation "xsimpl" "*" := xsimpl; auto_star.
+
+(** [xchange] helps rewriting in entailments. *)
+
+Lemma xchange_lemma : forall H1 H1',
+  H1 ==> H1' -> forall H H' H2,
+  H ==> H1 \* H2 ->
+  H1' \* H2 ==> H' ->
+  H ==> H'.
+Proof.
+  introv M1 M2 M3. applys himpl_trans M2. applys himpl_trans M3.
+  applys himpl_frame_l. applys M1.
+Qed.
+
+Tactic Notation "xchange" constr(M) :=
+  forwards_nounfold_then M ltac:(fun K =>
+    eapply xchange_lemma; [ eapply K | xsimpl | ]).
+
+
+(* ########################################################### *)
+(** ** Properties of [hwand] *)
+
+Lemma hwand_equiv : forall H0 H1 H2,
+  (H0 ==> H1 \-* H2) <-> (H1 \* H0 ==> H2).
+Proof using.
+  unfold hwand. iff M.
+  { rewrite hstar_comm. xchange M. rewrite hstar_hexists.
+    applys himpl_hexists_l. intros H. rewrite (hstar_comm H).
+    rewrite hstar_assoc. applys himpl_hstar_hpure_l. intros N.
+    rewrite hstar_comm. auto. }
+  { applys himpl_hexists_r H0. rewrite hstar_comm.
+    applys* himpl_hstar_hpure_r. }
+Qed.
+
+Lemma hwand_cancel : forall H1 H2,
+  H1 \* (H1 \-* H2) ==> H2.
+Proof using. intros. rewrite* <- hwand_equiv. Qed.
+
+Arguments hwand_cancel : clear implicits.
+
+
+(* ########################################################### *)
+(** ** Properties of [qwand] *)
+
+Lemma qwand_specialize : forall (v:val) (Q1 Q2:val->hprop),
+  (Q1 \--* Q2) ==> (Q1 v \-* Q2 v).
+Proof using.
+  intros. unfold qwand. applys himpl_hforall_l v. xsimpl.
+Qed.
+
+Lemma qwand_equiv : forall H Q1 Q2,
+      H ==> (Q1 \--* Q2)
+  <-> (Q1 \*+ H) ===> Q2.
+Proof using.
+  intros. iff M.
+  { intros x. xchange M. xchange (qwand_specialize x).
+    rewrite hstar_comm. applys (hwand_cancel (Q1 x)). }
+  { applys himpl_hforall_r. intros x. rewrite* hwand_equiv. }
+Qed.
+
+
+(* ########################################################### *)
+(** ** Properties of [hsingle] *)
+
+Lemma hstar_hsingle_same_loc : forall p v1 v2,
+  (p ~~> v1) \* (p ~~> v2) ==> \[False].
+Proof.
+  intros. unfold hsingle. intros h (h1&h2&E1&E2&D&E). false.
+  subst. applys* Fmap.disjoint_single_single_same_inv.
+Qed.
