omni/SepLogicOmniBig.v
@@ -1,0 +1,192 @@
+(****************************************************************
+* Imperative Lambda-calculus                                    *
+* Separation Logic on Omni-Big-Step                             *
+*****************************************************************)
+
+Set Implicit Arguments.
+Require Export SepLogicCommon OmniBig.
+
+Implicit Types f : var.
+Implicit Types b : bool.
+Implicit Types p : loc.
+Implicit Types n : int.
+Implicit Types v w r vf vx : val.
+Implicit Types t : trm.
+Implicit Types s : state.
+Implicit Types h : heap.
+Implicit Types H : hprop.
+Implicit Types Q : val->hprop.
+
+
+(* ########################################################### *)
+(* ########################################################### *)
+(* ########################################################### *)
+(** * Proof of the Frame Property for Omni-Big-Step *)
+
+Lemma omnibig_frame : forall h1 h2 t Q,
+  omnibig h1 t Q ->
+  Fmap.disjoint h1 h2 ->
+  omnibig (h1 \u h2) t (Q \*+ (= h2)).
+Proof using.
+  introv M HD. gen h2. induction M; intros;
+    try solve [ hint hstar_intro; constructors* ].
+  { rename M into M1, H into M2, IHM into IH1, H0 into IH2.
+    specializes IH1 HD. applys omnibig_let IH1. introv HK.
+    lets (h1'&h2'&K1'&K2'&KD&KU): HK. subst. applys* IH2. }
+  { rename H into M. applys omnibig_ref. intros p Hp.
+    rewrite Fmap.indom_union_eq in Hp. rew_logic in Hp.
+    destruct Hp as [Hp1 Hp2].
+    rewrite* Fmap.update_union_not_r. applys hstar_intro.
+    { applys* M. } { auto. } { applys* Fmap.disjoint_update_not_r. } }
+  { applys omnibig_get. { rewrite* Fmap.indom_union_eq. }
+    { rewrite* Fmap.read_union_l. applys* hstar_intro. } }
+  { applys omnibig_set. { rewrite* Fmap.indom_union_eq. }
+    { rewrite* Fmap.update_union_l. applys hstar_intro.
+      { auto. } { auto. } { applys* Fmap.disjoint_update_l. } } }
+  { applys omnibig_free. { rewrite* Fmap.indom_union_eq. }
+    { rewrite* Fmap.remove_disjoint_union_l. applys hstar_intro.
+      { auto. } { auto. } { applys* Fmap.disjoint_remove_l. } } }
+Qed.
+
+
+(* ########################################################### *)
+(* ########################################################### *)
+(* ########################################################### *)
+(** * Construction of Separation Logic *)
+
+(* ########################################################### *)
+(** ** Definition of Separation Logic triples *)
+
+Definition triple (t:trm) (H:hprop) (Q:val->hprop) : Prop :=
+  forall s, H s -> omnibig s t Q.
+
+
+(* ########################################################### *)
+(** ** Structural Rules *)
+
+Lemma triple_conseq : forall t H' Q' H Q,
+  triple t H' Q' ->
+  H ==> H' ->
+  Q' ===> Q ->
+  triple t H Q.
+Proof using. unfolds triple. introv M MH MQ HF. applys* omnibig_conseq. Qed.
+
+Lemma triple_frame : forall t H Q H',
+  triple t H Q ->
+  triple t (H \* H') (Q \*+ H').
+Proof.
+  introv M. intros h HF. lets (h1&h2&M1&M2&MD&MU): (rm HF).
+  subst. specializes M M1. applys omnibig_conseq.
+  { applys omnibig_frame M MD. } { xsimpl. intros h' ->. applys M2. }
+Qed.
+
+Lemma triple_hexists : forall t (A:Type) (J:A->hprop) Q,
+  (forall (x:A), triple t (J x) Q) ->
+  triple t (hexists J) Q.
+Proof using. introv M. intros h (x&Hh). applys M Hh. Qed.
+
+Lemma triple_hpure : forall t (P:Prop) H Q,
+  (P -> triple t H Q) ->
+  triple t (\[P] \* H) Q.
+Proof using.
+  introv M. intros h (h1&h2&M1&M2&D&U). destruct M1 as (M1&HP).
+  inverts HP. subst. rewrite Fmap.union_empty_l. applys~ M.
+Qed.
+
+
+(* ########################################################### *)
+(** ** Reasoning Rules for Terms *)
+
+Lemma triple_val : forall v H Q,
+  H ==> Q v ->
+  triple (trm_val v) H Q.
+Proof using. introv M Hs. applys* omnibig_val. Qed.
+
+Lemma triple_fix : forall f x t1 H Q,
+  H ==> Q (val_fix f x t1) ->
+  triple (trm_fix f x t1) H Q.
+Proof using. introv M Hs. applys* omnibig_fix. Qed.
+
+Lemma triple_if : forall (b:bool) t1 t2 H Q,
+  triple (if b then t1 else t2) H Q ->
+  triple (trm_if b t1 t2) H Q.
+Proof using. introv M Hs. applys* omnibig_if. Qed.
+
+Lemma triple_app_fix : forall v1 v2 f x t1 H Q,
+  v1 = val_fix f x t1 ->
+  triple (subst x v2 (subst f v1 t1)) H Q ->
+  triple (trm_app v1 v2) H Q.
+Proof using. introv E M Hs. applys* omnibig_app_fix. Qed.
+
+Lemma triple_let : forall x t1 t2 Q1 H Q,
+  triple t1 H Q1 ->
+  (forall v1, triple (subst x v1 t2) (Q1 v1) Q) ->
+  triple (trm_let x t1 t2) H Q.
+Proof using. introv M1 M2 Hs. applys* omnibig_let. Qed.
+
+
+(* ########################################################### *)
+(** ** Specification of Primitive Operations *)
+
+Lemma triple_div : forall n1 n2,
+  n2 <> 0 ->
+  triple (val_div n1 n2)
+    \[]
+    (fun r => \[r = val_int (Z.quot n1 n2)]).
+Proof using.
+  introv Hn2 Hs. applys* omnibig_div. inverts Hs. exists*. hnfs*.
+Qed.
+
+Lemma triple_rand : forall n,
+  n > 0 ->
+  triple (val_rand n)
+    \[]
+    (fun r => \[exists n1, r = val_int n1 /\ 0 <= n1 < n]).
+Proof using.
+  introv Hn2 Hs. applys* omnibig_rand. inverts Hs.
+  intros n1 Hn1. hnfs. exists*. hnfs*.
+Qed.
+
+Lemma triple_ref : forall v,
+  triple (val_ref v)
+    \[]
+    (fun r => \exists p, \[r = val_loc p] \* p ~~> v).
+Proof using.
+  intros. intros s1 K. applys omnibig_ref. intros p D.
+  inverts K. rewrite Fmap.update_empty. exists p.
+  rewrite hstar_hpure_l. split*. hnfs*.
+Qed.
+
+Lemma triple_get : forall v p,
+  triple (val_get p)
+    (p ~~> v)
+    (fun r => \[r = v] \* (p ~~> v)).
+Proof using.
+  intros. intros s K. inverts K. applys omnibig_get.
+  { applys* Fmap.indom_single. }
+  { rewrite hstar_hpure_l. split*. rewrite* Fmap.read_single. hnfs*. }
+Qed.
+
+Lemma triple_set : forall w p v,
+  triple (val_set (val_loc p) v)
+    (p ~~> w)
+    (fun r => (p ~~> v)).
+Proof using.
+  intros. intros s1 K. inverts K. applys omnibig_set.
+  { applys* Fmap.indom_single. }
+  { rewrite Fmap.update_single. hnfs*. }
+Qed.
+
+Lemma triple_free : forall p v,
+  triple (val_free (val_loc p))
+    (p ~~> v)
+    (fun r => \[]).
+Proof using.
+  intros. intros s1 K. inverts K. applys omnibig_free.
+  { applys* Fmap.indom_single. }
+  { rewrite* Fmap.remove_single. hnfs*. }
+Qed.
+
+(** For example proofs in Separation Logic, see the course:
+    Separation Logic Foundations, vol 6 of the Software Foundations series:
+    https://softwarefoundations.cis.upenn.edu/slf-current/index.html *)
